saw-core-coq/coq/handwritten/CryptolToCoq/CompRefl/Utils.v
@@ -1,7 +1,13 @@
 
-From Coq Require Import Lists.List.
-From Coq Require Import Bool.Bool.
+From Coq          Require Import Lists.List.
+From Coq          Require Import Bool.Bool.
+From Coq          Require Import Logic.Eqdep.
+From Coq          Require Import Logic.FunctionalExtensionality.
+From CryptolToCoq Require Import SAWCorePrelude.
+From CryptolToCoq Require Import CompM.
+
 Import ListNotations.
+Import EqNotations.
 
 Definition fromSum {A B C} (f : A -> C) (g : B -> C) (x : A + B) : C :=
   match x with
@@ -27,4 +33,42 @@ Proof.
   repeat (split; intros); subst; eauto.
   destruct H, b1; symmetry; eauto.
   destruct b2; symmetry; eauto.
+Qed.
+
+Definition eq_dep_eq1 {U P p x q y} (eq : eq_dep U P p x q y) : p = q :=
+  match eq with
+  | eq_dep_intro => eq_refl
+  end.
+
+Lemma f_eq_dep_2 :
+  forall U (P Q : U -> Type) R p q x y z w (f : forall p, P p -> Q p -> R p),
+    eq_dep U P p x q y -> eq_dep U Q p z q w -> eq_dep U R p (f p x z) q (f q y w).
+Proof.
+  intros.
+  destruct (eq_dep_eq1 H).
+  apply eq_dep_eq in H; apply eq_dep_eq in H0.
+  destruct H, H0; reflexivity.
+Qed.
+
+Lemma eq_dep_fun_ext {U A} {P : U -> Type} {p q} {f : A -> P p} {g : A -> P q} :
+  p = q -> (forall x, eq_dep U P p (f x) q (g x)) -> eq_dep U (fun i => A -> P i) p f q g.
+Proof.
+  destruct 1; intros.
+  enough (f = g) by (rewrite H0; eauto).
+  apply functional_extensionality; intro.
+  specialize (H x).
+  apply eq_dep_eq in H; eauto.
+Qed.
+
+Lemma eq_dep_bindM {A B C D : Set} {m1 m2} {k1 : A -> CompM C} {k2 : B -> CompM D} :
+  forall (H : eq_dep Set CompM A m1 B m2), C = D ->
+  (forall a, eq_dep Set CompM C (k1 a) D (k2 (rew eq_dep_eq1 H in a))) ->
+  eq_dep Set CompM C (m1 >>= k1) D (m2 >>= k2).
+Proof.
+  intros.
+  destruct (eq_dep_eq1 H); apply eq_dep_eq in H.
+  destruct H, H0.
+  apply eq_dep_fun_ext in H1; eauto.
+  apply eq_dep_eq in H1; simpl in H1.
+  rewrite H1; reflexivity.
 Qed.
